HAomega/Continuity.lean
@@ -191,6 +191,16 @@ theorem eval_tracked {Γ : List Ty} {τ : Ty} (t : Tm Γ τ) :
   | ord a b iha ihb =>
       intro E hE
       exact continuous2_binop Realizability.ordOf (iha E hE) (ihb E hE)
+  | hcut a b iha ihb =>
+      intro E hE
+      exact continuous2_binop Realizability.hydraStepN (iha E hE) (ihb E hE)
+  | hydra a b iha ihb =>
+      intro E hE
+      exact continuous2_binop Realizability.hydraSeqN (iha E hE) (ihb E hE)
+  | hord a ih =>
+      intro E hE
+      exact continuous2_binop (fun x _ ↦ Realizability.ordOfHydraN x)
+        (ih E hE) (continuous2_const 0)
   | tiRec s n ihs ihn =>
       intro E hE
       refine tracked_apply_nat _ (ihn E hE) fun j ↦ ?_
